theories/eris/lib/sampling/negative_binomial/interface.v
@@ -1,0 +1,130 @@
+From clutch.eris Require Export eris.
+From clutch.eris.lib.sampling Require Import utils. 
+From clutch.eris.lib.sampling.binomial Require Import interface.
+
+Section NegativeBinomialProbability.
+  
+  Definition negative_binom_prob (p q r k : nat) : R :=
+    (choose (k + r - 1) k * (p / (q + 1))^r * (1 - p  / (q + 1))^k)%R.
+
+  Lemma negative_binom_pos (p q r k : nat) : p ≤ (q + 1) → (0 <= negative_binom_prob p q r k)%R.
+  Proof.
+    intros Hpq.
+
+    rewrite /negative_binom_prob.
+    assert (0 <= q)%R by apply pos_INR.
+    repeat apply Rmult_le_pos.
+    { apply choose_pos. }
+    { apply pow_le, Rcomplements.Rdiv_le_0_compat; first apply pos_INR.
+      lra.
+    }
+    { apply pow_le.
+      rewrite -Rcomplements.Rminus_le_0 Rcomplements.Rle_div_l; last lra.
+      rewrite Rmult_1_l -INR_1 -plus_INR.
+      apply le_INR, Hpq.
+    }
+  Qed.
+      
+  Lemma negative_binom_prob_split : ∀ (p q r k : nat),
+    negative_binom_prob p q (r + 1) (k + 1)%nat =
+    ((1 - p / (q + 1)) * negative_binom_prob p q (r + 1) k
+     + (p / (q + 1)) * negative_binom_prob p q r (k + 1))%R.
+  Proof.
+    intros p q r k.
+    rewrite /negative_binom_prob.
+    replace (k + 1 + (r + 1) - 1) with (S (k + r)); last lia.
+    replace (k + 1 + r - 1) with (k + r); last lia.
+    replace (k + 1) with (S k); last lia.
+    replace (k + (r + 1) - 1) with (k + r); last lia.
+    rewrite -pascal' pow_add /=.
+    lra.
+  Qed.
+
+  Lemma negative_binom_prob_is_distr :
+    ∀ (p q r : nat),
+    p ≤ q + 1 →
+    SeriesC (negative_binom_prob p q r) = 1.
+  Admitted.
+  
+  Lemma ex_seriesC_negative_binom_prob :
+    ∀ (p q r : nat),
+    p ≤ q + 1 →
+    ex_seriesC (negative_binom_prob p q r).
+  Proof.
+    unfold ex_seriesC.
+    unfold is_seriesC.
+    intros p q r Hpq.
+    exists 1%R.
+    apply Series.is_series_Reals.
+    unfold infinite_sum.
+    intros ε Hε.
+  Admitted.
+
+End NegativeBinomialProbability.
+
+Class negative_binomial_spec `{!erisGS Σ} (negative_prog : val) :=
+  NegativeSpec
+  {
+    twp_negative_binomial_adv_comp :
+    ∀ (p q : nat),
+      (0 < p)%nat →
+      (p < q + 1)%nat →
+      ∀ (r : nat) (D : nat → R) (ε : R) (ε_term : R),
+      (0 < ε_term)%R →
+      (∀ (n : nat), 0 <= D n)%R →
+      SeriesC (λ k, (negative_binom_prob p q r k * D k)%R) = ε → ↯ ε_term -∗
+      ↯ ε -∗ WP negative_prog #() #p #q #r [{ v, ∃ (k : nat), ⌜v = #k⌝ ∗ ↯ (D k) }];
+
+    own_negative_tape (α : loc) (N M r : nat) (v : list nat) : iProp Σ;
+
+    twp_negative_tape :
+    ∀ (p q r : nat) (α : loc) (n : nat) (ns : list nat) (Φ : val → iProp Σ),
+    own_negative_tape α p q r (n::ns) -∗
+    (own_negative_tape α p q r ns -∗ Φ #n) -∗
+    WP negative_prog #lbl:α #p #q #r [{ Φ }];
+ 
+    twp_negative_binomial_presample :
+    ∀ (e : expr) (α : loc) (Φ : val → iProp Σ)
+      (p q r : nat) (ns : list nat) (ε : R),
+      (0 < p)%nat →
+      (p < q + 1)%nat →
+      (0 < ε)%R → 
+      to_val e = None →
+      ↯ ε ∗ own_negative_tape α p q r ns ∗
+      (∀ (i : nat), own_negative_tape α p q r (ns ++ [i]) -∗ WP e [{ Φ }])
+      ⊢  WP e [{ Φ }];
+  
+    twp_negative_binomial_planner :
+    ∀ (p q r : nat) (α : loc) (e : expr) (ε : nonnegreal)
+      (L_size L_sum : nat) (Φ : val → iProp Σ)
+      (prefix : list nat) (suffix : list nat → list nat) ,
+      (0 < p < q + 1)%nat →
+      0 < r →
+      to_val e = None →
+      (∀ (junk : list nat),
+         0 < length (suffix (prefix ++ junk)) <= L_size ∧ list_sum (suffix (prefix ++ junk)) ≤ L_sum) →
+      (0 < ε)%R →
+      ↯ ε ∗
+      own_negative_tape α p q r prefix ∗
+      ((∃ (junk : list nat),
+           own_negative_tape α p q r (prefix ++ junk ++ suffix (prefix ++ junk)))
+       -∗ WP e [{ Φ }])
+      ⊢ WP e [{ Φ }];
+
+    twp_negative_binomial_presample_adv_comp :
+    ∀ (p q : nat) (α : loc) (l : list nat) (e : expr) (Φ : val → iProp Σ),
+      0 < p →
+      p < (q + 1) →
+      to_val e = None →
+      ∀ (r : nat) (D : nat → R) (ε : R) (ε_term : R),
+      (0 < ε_term)%R →
+      (∀ (n : nat), 0 <= D n)%R →
+      SeriesC (λ k, (negative_binom_prob p q r k * D k)%R) = ε →
+      ↯ ε_term ∗
+      ↯ ε ∗
+      own_negative_tape α p q r l ∗
+      (∀ (n : nat),
+         ↯ (D n) -∗
+         own_negative_tape α p q r (l ++ [n]) -∗ WP e [{ Φ }]) ⊢
+      WP e [{ Φ }]
+  }.
